Innleveringsklar

src/v0.3/acceptor.dfy
@@ -1,70 +1,73 @@
-class Acceptor<T(==)>
-{
-  var promise:  int;
-  var accepted: Accepted<T>;
-
-  constructor (value: T)
-    modifies this;
-	ensures valid();
+module Acceptor {
+  class SingleAcceptor<T(==)>
   {
-    promise  := -1;
+    var promise:  int;
+    var accepted: Accepted<T>;
+
+    constructor (value: T)
+    modifies this;
+    ensures valid();
+    {
+    promise  := 0;
     accepted := new Accepted(value);
-  }
+    }
 
-  method Prepare(round: int, value: T) returns (ok: bool, acp: Accepted<T>)
-	requires valid();
+    method Prepare(round: int, value: T) returns (acp: Accepted<T>)
+    requires valid();
     modifies this;
-	ensures valid() && promise >= round;
-  {
-	acp := accepted;
-	ok  := false;
+    ensures valid() && if acp != null
+      then promise == round > acp.round
+      else promise >= round;
+    {
     // is the round at least as new as our promise
-	// and we have not already accepted it?
+    // and we have not already accepted it?
     if round >= promise && round != accepted.round {
       promise := round;
-	  assert promise > accepted.round;
-	  // TODO: store state?
-	  ok := true;
+      // TODO: store state?
+      acp := accepted;
     }
-  }
+    acp := null;
+    }
 
-  method Accept(round: int, value: T) returns (ok: bool, acp: Accepted<T>)
-	requires valid();
+    method Accept(round: int, value: T) returns (acp: Accepted<T>)
+    requires valid();
     modifies this, accepted;
-	ensures valid() && promise >= round;
-  {
-	acp := accepted;
-	ok  := false;
+    ensures valid() && promise >= round && if acp != null
+      then acp.round == round == promise && acp.value == value
+      else round < promise;
+    {
     // is the round at least as new as our promise?
     if round >= promise {
       promise        := round;
       accepted.round := round;
       accepted.value := value;
-	  // TODO: store state
-	  ok := true;
+      // TODO: store state
+      acp := accepted;
     }
-  }
+    acp := null;
+    }
 
-  method Get() returns (rnd: int, acp: int, val: T)
+    method Get() returns (rnd: int, acp: int, val: T)
     requires valid();
-  {
-	rnd := promise;
-	acp := accepted.round;
-	val := accepted.value;
+    {
+    rnd := promise;
+    acp := accepted.round;
+    val := accepted.value;
+    }
+
+    predicate valid()
+    reads this, accepted;
+    { accepted != null && promise >= accepted.round }
   }
 
-  predicate valid()
-    reads this, accepted;
-  { accepted != null && promise >= accepted.round }
-}
+  class Accepted<T(==)>
+  {
+    var round: int;
+    var value: T;
 
-class Accepted<T(==)>
-{
-  var round: int;
-  var value: T;
-
-  constructor (val: T)
+    constructor (val: T)
     modifies this;
-    ensures round == -1; // yes, this has to be explicitly stated!
-  { round := -1; value := val; }
+    ensures round == 0; // yes, this has to be explicitly stated!
+    { round := 0; value := val; }
+  }
 }
