src/v0.3/replica.dfy
@@ -1,1 +1,169 @@
-import opened Proposer 
+module Replica {
+	import opened Proposer
+	import opened Acceptor
+	import opened Learner
+
+	trait EndPoint {
+		function Equals(other: EndPoint): bool
+			reads this;
+			ensures this == other;
+	}
+
+	class Replica<T(==), EndPoint(==)> {
+
+		var self:      EndPoint;
+		var val:       T;
+		var consensus: int;
+		var majority:  int;
+		var proposer:  SingleProposer<T>;
+		var acceptor:  SingleAcceptor<T>;
+		var learner:   SingleLearner<T>;
+		var acceptors: map<int, EndPoint>;
+		var learners:  map<int, EndPoint>;
+
+		ghost var ghostacp: map<int, SingleAcceptor<T>>;
+
+		constructor (id: int, roles: int, val: T, self: EndPoint)
+		// roles are bitpattern [p.a.l] e.g 111 for all roles
+			requires this.proposer == null && this.acceptor == null && this.learner == null;
+			modifies this, this.proposer, this.learner;
+			ensures acceptor == null || acceptor.valid();
+			ensures proposer == null || proposer.valid();
+		{
+			consensus := 0;
+			var state_pro := false; // the state of this.proposer
+			var state_acp := false; // the state of this.acceptor
+			// false ==> null, true ==> valid
+			this.self := self;
+			this.val  := val;
+			if ( roles >= 100 ) {
+				proposer := new SingleProposer<T>( -1, val );
+				state_pro := true;
+				assert proposer.valid();
+			}
+			assert acceptor == null;
+			var roles := roles % 100;
+			if ( roles >= 10 ) {
+				acceptor := new SingleAcceptor<T>( val );
+				state_acp := true;
+				assert acceptor != null && acceptor.valid();
+				AddAcceptor( id, self, state_pro, state_acp );
+				assert acceptor != null && acceptor.valid();
+			}
+			assert proposer == null || proposer.valid();
+			roles := roles % 10;
+			if (roles >= 1) {
+				learner := new SingleLearner<T>();
+				AddLearner( id, self, state_acp );
+			}
+		}
+
+		method Promise(id: int, acp_round: int, acp_value: T)
+			returns (ok: bool, largest: int, val: T)
+			requires valid( proposer != null, acceptor != null);
+			requires proposer != null ==> (
+				proposer.valid()
+				// acceptors with equal round have equal value
+				&& (acp_round == proposer.largest ==> acp_value == proposer.value)
+				&& (acp_round in proposer.acceptors ==> proposer.acceptors[acp_round] == acp_value)
+			);
+			modifies this.proposer;
+			ensures  proposer == null || ok ==> proposer.round >= acp_round;
+			ensures  valid( proposer != null, acceptor != null);
+		{
+			ok, largest, val := false, -1, acp_value;
+			if proposer != null {
+				ok, largest, val := proposer.Promise(id, acp_round, acp_value);
+				assert ok ==> largest >= acp_round;
+			}
+			return ok, largest, val;
+		}
+
+		method Prepare(round: int, value: T) returns (acp: Accepted<T>)
+			requires acceptor == null || acceptor.valid();
+			modifies this, this.acceptor;
+			ensures acceptor == null || acceptor.promise >= round;
+		{
+			if acceptor != null {
+				acp := acceptor.Prepare(round, value);
+				if acp != null {
+					this.val := acp.value;
+				}
+			}
+		}
+
+		method Accept(round: int, value: T) returns (acp: Accepted<T>)
+			requires acceptor == null || acceptor.valid();
+			modifies this, this.acceptor;
+			modifies if this.acceptor != null then this.acceptor.accepted else null;
+			ensures acceptor == null || acceptor.promise >= round;
+		{
+			if acceptor != null {
+				acp := acceptor.Accept(round, value);
+				if acp != null && acp.round > round {
+					assert acp.round == round;
+					assert acp.value == value;
+					this.consensus := this.consensus + 1;
+				}
+			}
+		}
+
+		method Learn(id: int, round: int, value: T) returns (learned: bool, ret: T)
+			modifies this.learner;
+			// the final proof
+			ensures if learned
+			  then consensus >= majority
+			  else consensus < majority;
+		{
+			if learner != null {
+				learned, ret := learner.Learn(id, round, value);
+			}
+		}
+
+		method AddAcceptor(id: int, addr: EndPoint, state_pro: bool, state_acp: bool)
+			requires valid(state_pro, state_acp);
+			modifies this, this.proposer, this.learner;
+			ensures  valid(state_pro, state_acp);
+		{
+			acceptors := acceptors[id := addr];
+			Configure( |acceptors|, state_pro, state_acp );
+		}
+
+		method AddLearner(id: int, addr: EndPoint, state_acp: bool)
+			requires if state_acp
+				then acceptor != null && acceptor.valid()
+				else acceptor == null;
+			modifies this;
+			ensures  if state_acp
+				then acceptor != null && acceptor.valid()
+				else acceptor == null;
+		{ learners := learners[id := addr]; }
+
+		method Configure(num_acps: int, state_pro: bool, state_acp: bool)
+			requires valid(state_pro, state_acp);
+			modifies this, this.proposer, this.learner;
+			ensures  valid(state_pro, state_acp);
+		{
+			this.majority := num_acps/2 + 1;
+			if state_pro {
+				proposer.SetMajority( majority );
+			}
+			// TODO: re-evaluate proposer's |prepared| because we might not get more promises!
+			if (learner  != null) {
+				learner.majority  := this.majority;
+			}
+		}
+
+		predicate valid(state_pro: bool, state_acp: bool)
+			reads this, this.proposer, this.acceptor,
+				if this.acceptor != null then this.acceptor.accepted else null;
+		{
+			(if state_pro
+				then proposer != null && proposer.valid()
+				else proposer == null)
+			&& (if state_acp
+				then acceptor != null && acceptor.valid()
+				else acceptor == null)
+		}
+	}
+}
